DiagonaLean/UTMHalt/README.md
@@ -1,0 +1,14 @@
+```
+Copyright (c) 2026 Akhilesh Balaji. All rights reserved.
+Released under Apache 2.0 license as described in the file LICENSE.
+Authors: Akhilesh Balaji
+```
+# `UTMHalt`: The Universal Turing Machine Halting Problem
+## Problem Statement
+Given an encoding `⟪ M ⟫ w` of a TM `M` and input `w`, does `U`, a Turing Machine satisfying `IsWeaklyUniversal`, halt on `⟪ M ⟫ w`?
+
+A machine `U` is weakly universal with respect to `pair` if for every TM `M`
+and input `w`:
+```
+Halts M w  ↔  Halts U (pair (encodeBoolTM M) w)
+```
